

$$y = x^2 - 2x - 3$$

$$\Delta = -2^2 - 4 \cdot 1 \cdot (-3)$$

$$\Delta = 4 - (-12)$$

$$\Delta = 16$$

$\Delta > 0 = 2$ RAÍZES

$$x = \frac{-(-2) + \sqrt{16}}{2 \cdot 1} = \frac{2 + 4}{2} = \frac{6}{2} = \textcircled{3}$$

$$y = \frac{-(-2) - \sqrt{16}}{2 \cdot 1} = \frac{2 - 4}{2} = \frac{-2}{2} = \textcircled{-1}$$

máximo ou mínimo $x = \frac{-b}{2a} = \frac{-(-2)}{2 \cdot 1} = \frac{2}{2} = \textcircled{1}$

$$y = \frac{-\Delta}{4 \cdot a} = \frac{-16}{4 \cdot 1} = \frac{-16}{4} = \textcircled{-4}$$

$$y = -x^2 + 2x - 4$$

$$\Delta = 2^2 - 4 \cdot (-1) \cdot (-4)$$

$$\Delta = 4 - (16)$$

$$\Delta = -12$$

Sem Raízes
 $\Delta < 0$

$$x = \frac{-b}{2a} = \frac{-2}{2 \cdot (-1)} = \frac{-2}{-2} = \textcircled{1}$$

$$y = \frac{-\Delta}{4 \cdot a} = \frac{-(-12)}{4 \cdot (-1)} = \frac{12}{-4} = \textcircled{-3}$$

$$y = 4 - x^2$$

$$\Delta = 1^2 - 4 \cdot (-1) \cdot 4$$

$$\Delta = 1 - (-16)$$

$$\Delta = 17$$

$$\frac{-1 + \sqrt{17}}{2 \cdot (-1)} = \frac{-1 + \sqrt{17}}{-2} //$$

$$x = \frac{-b}{2a} = \frac{-1}{2 \cdot (-1)} = \frac{-1}{-2} = \textcircled{0}$$

$$y = \frac{-\Delta}{4 \cdot a} = \frac{-17}{4 \cdot (-1)} = \frac{-17}{-4} = \textcircled{4}$$

$$y = 4x^2 + 20x + 25$$

$$\Delta = b^2 - 4 \cdot (4) \cdot 25$$

$$\Delta = 400 - 400$$

$$\Delta = 0$$

Única Raiz
 $\Delta = 0$

$$\frac{-20 + 0}{2 \cdot 4} = \frac{-20}{8} = -2.5$$

$$x = \frac{-b}{2a} = \frac{-20}{2 \cdot 4} = -2.5$$

$$y = \frac{-\Delta}{4 \cdot a} = \frac{-0}{4 \cdot 4} = \frac{0}{8} = 0$$

$$\begin{array}{ccc} a & b & c \\ \Delta = (-5)^2 - 4 \cdot 1 \cdot 0 \\ \Delta = 25 - 0 = 25 \end{array}$$

$$\begin{array}{l} \frac{-b \pm \sqrt{\Delta}}{2a} = \frac{-(-5) \pm \sqrt{25}}{2 \cdot 1} = \frac{5 \pm 5}{2} = 5 \\ \frac{-(-5) - \sqrt{25}}{2 \cdot 1} = \frac{5 - 5}{2} = \frac{0}{2} = 0 \end{array}$$

$$x = \frac{-b}{2a} = \frac{-(-5)}{2 \cdot 1} = \frac{5}{2} = 2,5$$

$$y = \frac{-\Delta}{4a} = \frac{-25}{4 \cdot 1} = -\frac{25}{4} = -6,25$$

$$y = -x^2 \quad \begin{array}{ccc} 0 & x & 0 \\ a & b & c \end{array}$$

$$\Delta = 0^2 - 4 \cdot (-1) \cdot 0$$

$$\Delta = 0 - 0$$

$$\Delta = 0$$

$$\frac{-0 \pm 0}{2 \cdot (-1)} = \frac{0}{2} = 0$$

~~1/2~~